QsADTs: add tuple copy

Bedrock/Platform/Facade/examples/ArrayTupleF.v
@@ -35,8 +35,12 @@ Defined.
 
 Definition newS := newS tuple 7.
 Definition deleteS := deleteS tuple 6.
+Definition copyS := copyS tuple 11.
 Definition getS := getS tuple 0.
 Definition setS := setS tuple 0.
+
+Definition agreeUpto (ls1 ls2 : list W) (pos : nat) :=
+  forall i, (i < pos)%nat -> Array.selN ls1 i = Array.selN ls2 i.
 
 Definition m := bimport [[ "malloc"!"malloc" @ [mallocS], "malloc"!"free" @ [freeS] ]]
   bmodule "ListSeq" {{
@@ -59,6 +63,35 @@ Definition m := bimport [[ "malloc"!"malloc" @ [mallocS], "malloc"!"free" @ [fre
       Return 0
     end
 
+    with bfunction "copy"("extra_stack", "self", "len", "copy", "i", "tmp", "tmp2") [copyS]
+      "copy" <-- Call "malloc"!"malloc"(0, "len")
+      [Al ls,
+       PRE[V, R] tuple ls (V "self") * [| length ls = wordToNat (V "len") |]
+         * R =?> wordToNat (V "len") * [| R <> 0 |] * [| freeable R (wordToNat (V "len")) |]
+       POST[R'] tuple ls (V "self") * tuple ls R'];;
+
+      Note [make_array];;
+      "i" <- 0;;
+      [Al ls1, Al ls2,
+       PRE[V] tuple ls1 (V "self") * tuple ls2 (V "copy") * [| agreeUpto ls1 ls2 (wordToNat (V "i")) |]
+         * [| length ls1 = wordToNat (V "len") |] * [| length ls2 = wordToNat (V "len") |]
+       POST[R] [| R = V "copy" |] * tuple ls1 (V "self") * tuple ls1 (V "copy")]
+      While ("i" < "len") {
+        Assert [Al ls1, Al ls2,
+                PRE[V] tuple ls1 (V "self") * tuple ls2 (V "copy") * [| agreeUpto ls1 ls2 (wordToNat (V "i")) |]
+                  * [| length ls1 = wordToNat (V "len") |] * [| length ls2 = wordToNat (V "len") |]
+                  * [| (V "i" < natToW (length ls1))%word |] * [| (V "i" < natToW (length ls2))%word |]
+                POST[R] [| R = V "copy" |] * tuple ls1 (V "copy") * tuple ls1 (V "self")];;
+
+        "tmp" <- 4 * "i";;
+        "tmp2" <-* "self" + "tmp";;
+        "copy" + "tmp" *<- "tmp2";;
+        "i" <- "i" + 1
+      };;
+
+      Return "copy"
+    end
+
     with bfunction "get"("extra_stack", "self", "pos") [getS]
       "pos" <- 4 * "pos";;
       "pos" <-* "self" + "pos";;
@@ -73,6 +106,141 @@ Definition m := bimport [[ "malloc"!"malloc" @ [mallocS], "malloc"!"free" @ [fre
   }}.
 
 Local Hint Extern 1 (@eq W _ _) => words.
+
+Lemma agreeUpto_O : forall ls1 ls2, agreeUpto ls1 ls2 0.
+Proof.
+  unfold agreeUpto; intros; omega.
+Qed.
+
+Hint Resolve agreeUpto_O.
+
+Lemma freeable_cong : forall p n n',
+  freeable p n'
+  -> n = n'
+  -> freeable p n.
+Proof.
+  congruence.
+Qed.
+
+Hint Immediate freeable_cong.
+
+Lemma selN_updN_ne : forall v a n n',
+  n <> n'
+  -> Array.selN (Array.updN a n v) n' = Array.selN a n'.
+Proof.
+  induction a; destruct n, n'; simpl; intuition.
+Qed.
+
+Lemma agreeUpto_S : forall ls1 ls2 n,
+  agreeUpto ls1 ls2 (wordToNat n)
+  -> n < natToW (length ls2)
+  -> goodSize (length ls2)
+  -> agreeUpto ls1 (Array.upd ls2 n (Array.sel ls1 n)) (wordToNat (n ^+ $1)).
+Proof.
+  unfold agreeUpto; intros.
+  rewrite wordToNat_wplus in H2.
+  change (wordToNat $1) with 1 in H2.
+  assert (i < wordToNat n \/ i = wordToNat n)%nat by omega; intuition subst.
+  rewrite H by assumption.
+
+  unfold Array.upd.
+  rewrite selN_updN_ne by omega; auto.
+
+  unfold Array.upd.
+  rewrite selN_updN_eq; auto.
+  apply lt_goodSize'; auto.
+  unfold natToW; rewrite natToWord_wordToNat; auto.
+  change (wordToNat $1) with 1.
+  eapply goodSize_weaken; eauto.
+
+  assert (wordToNat n < length ls2)%nat; try omega.
+  apply lt_goodSize'; auto.
+  unfold natToW; rewrite natToWord_wordToNat; auto.
+Qed.
+
+Hint Extern 1 (agreeUpto _ (Array.upd _ _ _) _) =>
+  eapply agreeUpto_S; [ eassumption | eassumption | solve [ eauto 7 ] ].
+
+Lemma bound_nat : forall i len n,
+  i < len
+  -> n = wordToNat len
+  -> i < natToW n.
+Proof.
+  intros; subst.
+  unfold natToW; rewrite natToWord_wordToNat; auto.
+Qed.
+
+Hint Immediate bound_nat.
+
+Lemma agreeUpto_total : forall ls1 ls2 (i : W) len,
+  agreeUpto ls1 ls2 (wordToNat i)
+  -> len <= i
+  -> length ls1 = wordToNat len
+  -> length ls2 = wordToNat len
+  -> ls1 = ls2.
+Proof.
+  induction ls1; destruct ls2; simpl; intuition.
+
+  assert (Hgt : (wordToNat i > 0)%nat).
+  unfold wlt in H0.
+  destruct (wordToNat i) eqn:Heq.
+  rewrite wordToN_nat in H0.
+  rewrite Heq in H0; simpl in H0.
+  exfalso; apply H0.
+  rewrite wordToN_nat.
+  destruct (wordToNat len); nomega.
+  omega.
+
+  assert (Hle : $1 <= i).
+  unfold wlt.
+  change (wordToN $1) with 1%N.
+  nomega.
+
+  assert (Hlen : $1 <= len).
+  unfold wlt.
+  change (wordToN $1) with 1%N.
+  pre_nomega.
+  change (Pos.to_nat 1) with 1.
+  destruct (wordToNat len); omega.
+
+  f_equal.
+
+  specialize (H 0); intuition idtac.
+
+  apply IHls1 with (i ^- $1) (len ^- $1).
+  do 2 intro.
+  specialize (H (S i0)).
+  apply H.
+  rewrite wordToNat_wminus in H3 by assumption.
+  change (wordToNat $1) with 1 in *.
+  omega.
+
+  unfold wlt; intro.
+  apply Nlt_out in H3.
+  autorewrite with N in *.
+  repeat rewrite wordToNat_wminus in H3 by assumption.
+  nomega.
+
+  rewrite wordToNat_wminus by assumption.
+  change (wordToNat $1) with 1; omega.
+  rewrite wordToNat_wminus by assumption.
+  change (wordToNat $1) with 1; omega.
+Qed.
+
+Lemma agreeUpto_total_himp : forall ls1 ls2 (i : W) len specs p,
+  agreeUpto ls1 ls2 (wordToNat i)
+  -> len <= i
+  -> length ls1 = wordToNat len
+  -> length ls2 = wordToNat len
+  -> himp specs (array ls2 p) (array ls1 p).
+Proof.
+  intros.
+  replace ls2 with ls1.
+  reflexivity.
+  eauto using agreeUpto_total.
+Qed.
+
+Hint Immediate agreeUpto_total_himp.
 
 Theorem ok : moduleOk m.
 Proof.
