Bedrock/Platform/Facade/examples/TupleF.v
@@ -13,6 +13,11 @@ Section adt.
     PRE[V] P ls (V "self") * [| length ls = wordToNat (V "len") |] * mallocHeap 0
     POST[R] [| R = $0 |] * mallocHeap 0.
 
+  Definition copyS := SPEC("extra_stack", "self", "len") reserving res
+    Al ls,
+    PRE[V] P ls (V "self") * [| length ls = wordToNat (V "len") |] * [| $2 <= V "len" |] * mallocHeap 0
+    POST[R] P ls (V "self") * P ls R * mallocHeap 0.
+
   Definition getS := SPEC("extra_stack", "self", "pos") reserving res
     Al ls,
     PRE[V] P ls (V "self") * [| V "pos" < natToW (length ls) |] * mallocHeap 0
